More wip

src/Parsers/BooleanRecognizerCorrect.v
@@ -57,8 +57,8 @@ Section sound.
           := forall prod prods, str_matches_productions prod prods = true
                                 -> parse_of _ G str (prod::prods).
 
-        Definition str_matches_productions_completeT
-          := forall valid (H_sub : H_subT valid) prod prods,
+        Definition str_matches_productions_completeT P
+          := forall valid (H_sub : P valid) prod prods,
                minimal_parse_of _ G initial_productions_data is_valid_productions remove_productions valid str (prod::prods)
                -> str_matches_productions prod prods = true.
 
@@ -81,15 +81,14 @@ Section sound.
         Defined.
 
         Lemma parse_item_complete
-              valid
-              (H_sub : H_subT valid)
-              (str_matches_productions_complete : str_matches_productions_completeT)
+              valid Pv
+              (H_sub : forall p, Pv (remove_productions valid p))
+              (str_matches_productions_complete : str_matches_productions_completeT Pv)
               (it : item CharType)
         : minimal_parse_of_item _ G initial_productions_data is_valid_productions remove_productions valid str it
           -> parse_item String G str str_matches_productions it = true.
         Proof.
           unfold parse_item, str_matches_productions_completeT in *.
-          subst H_subT; simpl in *.
           repeat match goal with
                    | _ => intro
                    | _ => reflexivity
@@ -97,7 +96,7 @@ Section sound.
                    | [ |- _ = true ] => apply bool_eq_correct
                    | [ H : context[?E] |- context[match ?E with _ => _ end] ] => destruct E
                    | [ H : minimal_parse_of _ _ _ _ _ _ _ [] |- _ ] => solve [ inversion H ]
-                   | _ => solve [ eauto using sub_productions_listT_remove_2 ]
+                   | _ => solve [ eauto ]
                end.
         Qed.
       End item.
@@ -133,8 +132,8 @@ Section sound.
                @parse_productions str pf prod prods = true
                -> parse_of _ G str (prod::prods).
 
-        Definition parse_productions_completeT
-          := forall valid (H_sub : H_subT valid) str pf prod prods,
+        Definition parse_productions_completeT P
+          := forall valid (H_sub : P valid) str pf prod prods,
                minimal_parse_of _ G initial_productions_data is_valid_productions remove_productions valid str (prod::prods)
                -> @parse_productions str pf prod prods = true.
 
@@ -200,17 +199,20 @@ Section sound.
         Defined.
 
         Lemma parse_production_complete
-              valid
-              (H_sub : H_subT valid)
-              (parse_productions_complete : parse_productions_completeT)
-              (split_string_for_production_complete : forall valid1 (H1_sub : H_subT valid1) valid2 (H2_sub : H_subT valid2) str pf prod, @split_list_completeT valid1 valid2 str pf (split_string_for_production str prod) prod)
+              valid Pv
+              (H_sub : Pv valid)
+              (Hv_init : Pv initial_productions_data)
+              (Hv_init_rem : forall p, Pv (remove_productions initial_productions_data p))
+              (Hv_rem : forall p, Pv (remove_productions valid p))
+              (parse_productions_complete : parse_productions_completeT Pv)
+              (split_string_for_production_complete : forall valid1 (H1_sub : Pv valid1) valid2 (H2_sub : Pv valid2) str pf prod, @split_list_completeT valid1 valid2 str pf (split_string_for_production str prod) prod)
               (str : String) (pf : str ≤s str0)
               (prod : production CharType)
         : minimal_parse_of_production _ G initial_productions_data is_valid_productions remove_productions valid str prod
           -> parse_production G split_string_for_production split_string_for_production_correct parse_productions pf prod = true.
         Proof.
           change (forall str0 prod, split_list_correctT str0 (split_string_for_production str0 prod)) in split_string_for_production_correct.
-          revert valid H_sub str pf; induction prod;
+          revert valid H_sub Hv_rem str pf; induction prod;
           repeat match goal with
                    | _ => intro
                    | _ => progress simpl in *
@@ -260,7 +262,7 @@ Section sound.
                    | _ => split
                    | [ |- (_ && _)%bool = true ] => apply Bool.andb_true_iff
                    | _ => eapply parse_item_complete; [..| eassumption ];
-                          unfold H_subT; simpl;
+                          try unfold H_subT; simpl;
                           try eassumption; try reflexivity;
                           hnf in parse_productions_complete |- *;
                           solve [ apply parse_productions_complete
@@ -349,10 +351,13 @@ Section sound.
           Defined.
 
           Lemma parse_productions_step_complete
-                (parse_productions_complete : parse_productions_completeT parse_productions)
+                valid Pv
+                (H_sub : Pv valid)
+                (Hv_init : Pv initial_productions_data)
+                (Hv_init_rem : forall p, Pv (remove_productions initial_productions_data p))
+                (Hv_rem : forall p, Pv (remove_productions valid p))
+                (parse_productions_complete : parse_productions_completeT parse_productions Pv)
                 (split_string_for_production_complete : forall valid1 valid2 str pf prod, @split_list_completeT str0 valid1 valid2 str pf (split_string_for_production str prod) prod)
-                valid
-                (H_sub : H_subT valid)
                 (str : String) (pf : str ≤s str0) (prod : production CharType) (prods : productions CharType)
           : minimal_parse_of _ G initial_productions_data is_valid_productions remove_productions valid str (prod::prods)
             -> parse_productions_step G split_string_for_production split_string_for_production_correct parse_productions pf (prod::prods) = true.
@@ -362,7 +367,7 @@ Section sound.
             induction prods; simpl; auto.
             { parse_productions_step_t.
               left; eapply parse_production_complete; [..| eassumption ];
-              solve [ trivial ]. }
+              solve [ eassumption | trivial ]. }
             { parse_productions_step_t;
               match goal with
                 | [ H : forall prod, minimal_parse_of _ _ _ _ _ _ ?s (prod::_) -> _,
@@ -471,8 +476,22 @@ Section sound.
           Defined.
 
           Lemma parse_productions_or_abort_helper_complete
+                Pv
                 (p : String * productions_listT) (str : String)
-                (H_sub : sub_productions_listT is_valid_productions (snd p) initial_productions_data)
+                (H_sub : Pv (snd p))
+                (Hv_init : Pv initial_productions_data)
+                (Hv_rem : forall p' v, Pv v -> Pv (remove_productions v p'))
+                (Hv_expand
+                 : forall str p' valid,
+                     Pv valid
+                     -> minimal_parse_of
+                          String G initial_productions_data
+                          is_valid_productions remove_productions valid str
+                          p'
+                     -> minimal_parse_of
+                          String G initial_productions_data
+                          is_valid_productions remove_productions initial_productions_data str
+                          p')
                 (split_string_for_production_complete : forall valid0 valid1 str0 pf prod, @split_list_completeT str valid0 valid1 str0 pf (split_string_for_production str0 prod) prod)
                 (pf : str ≤s fst p)
                 (prod : production CharType)
@@ -493,13 +512,13 @@ Section sound.
             { match goal with
                 | [ |- context[if lt_dec ?a ?b then _ else _] ] => destruct (lt_dec a b)
               end.
-              { eapply parse_productions_step_complete; try eassumption; [].
+              { eapply parse_productions_step_complete;
+                try solve [ eassumption | instantiate; intros; eauto ]; [].
                 intros valid H_sub0 str0 pf0 prod0 prods0 H'; eapply IHr;
-                try first [ exact H' | eassumption | reflexivity ].
+                try solve [ exact H' | eassumption | reflexivity | simpl; eauto ].
                 { left; assumption. }
                 { intros; apply split_string_for_production_complete.
-                  etransitivity; eassumption. }
-                { eapply expand_minimal_parse_of; [..| eassumption ]; trivial. } }
+                  etransitivity; eassumption. } }
               { let ivp := match goal with |- context[is_valid_productions ?x ?y] => constr:(is_valid_productions x y) end in
                 set (ivp' := ivp);
                   assert (ivp = ivp') by reflexivity;
@@ -509,17 +528,12 @@ Section sound.
                   hnf in pf.
                   apply or_to_sumbool in pf.
                   destruct pf as [ pf | pf ]; [ exfalso; hnf in *; solve [ auto ] | subst ].
-                  Print parse_productions_step.
-
-                  eapply parse_productions_step_complete; try eassumption.
-                  hnf.
-
+                  eapply parse_productions_step_complete;
+                    try solve [ eassumption | instantiate; intros; eauto ]; [].
                   intros valid H_sub0 str0 pf0 prod0 prods0 H'; eapply IHr;
-                  try first [ exact H' | eassumption ].
+                  try solve [ exact H' | eassumption | simpl; eauto ].
                   { right; split; trivial; simpl.
                     apply remove_productions_dec; assumption. }
-                  { subst H_subT; simpl in *.
-                    eauto using sub_productions_listT_remove_2. }
                   { intros; apply split_string_for_production_complete.
                     etransitivity; eassumption. }
                   { simpl.
